Day 2

problems/2/Problem2.dfy
@@ -1,9 +1,65 @@
+include "../../parser/split.dfy"
+include "../../parser/parseInt.dfy"
 module Problem2 {
+    import opened Split
+    import opened ParseInt
+    import opened Std.Collections.Seq
+
+    method parseInput(input: string) returns (ss: seq<seq<int>>) {
+        var data := splitOnBreak(input);
+        ss := Map(s => Map(Integer, split(s, " ")), Filter((s: string) => s != "", data));
+    }
+
+    predicate Increasing(s: seq<int>) {
+        if |s| <= 1 then true else s[0] <= s[1] && Increasing(s[1..])
+    }
+
+    predicate Increasing2(s: seq<int>) {
+        forall i :: 0 <= i < |s| - 1 ==> s[i] <= s[i + 1]
+    }
+
+    predicate Decreasing(s: seq<int>) {
+        if |s| <= 1 then true else s[0] >= s[1] && Decreasing(s[1..])
+    }
+
+    predicate Decreasing2(s: seq<int>) {
+        forall i :: 0 <= i < |s| - 1 ==> s[i] >= s[i + 1]
+    }
+
+    function abs(x: int): int {
+        if x < 0 then -x else x
+    }
+
+    predicate DiffersBy(ss: seq<int>) {
+        forall i :: 0 <= i < |ss| - 1 ==> 1 <= abs(ss[i] - ss[i + 1]) <= 3
+    }
+
+    predicate SafeReport(ss: seq<int>) {
+        // (Increasing(ss) || Decreasing(ss)) && DiffersBy(ss)
+        (Increasing2(ss) || Decreasing2(ss)) && DiffersBy(ss)
+    }
+
+    predicate SafeWithOneRemoved(ss: seq<int>) {
+        exists i :: 0 <= i < |ss|  && SafeReport(ss[0..i] + ss[i + 1..])
+    }
+
     method problem2_1(input: string) returns (x: int) {
-        return 3;
+        var data := parseInput(input);
+        x := 0;
+        for i := 0 to |data| {
+            if SafeReport(data[i]) {
+                x := x + 1;
+            }
+        }
     }
 
     method problem2_2(input: string) returns (x: int) {
-        return 4;
+        var data := parseInput(input);
+        x := 0;
+        for i := 0 to |data| {
+            if SafeReport(data[i]) || SafeWithOneRemoved(data[i]) {
+                x := x + 1;
+            }
+        }
     }
 }
